\problemset{Бета-редукция}

\begin{problem}
Выполнить бета-редукцию λ-терма ((λa.(λb.b b) (λb.b b)) b) ((λc.(c b)) (λa.a))
\end{problem}
\begin{solution}
((λa.(λb.b b) (λb.b b)) b) ((λc.(c b)) (λa.a)) $\underset{\beta}{\longrightarrow}$ (λb.b b) (λb.b b) ((λc.(c b)) (λa.a)) $\underset{\beta}{\longrightarrow}$ 
(λb.b b) (λb.b b) (λa.a) b $\underset{\beta}{\longrightarrow}$ (λb.b b) (λb.b b) b $\underset{\beta}{\longrightarrow}$ (λb.b b) b b $\underset{\beta}{\longrightarrow}$ b b b
\end{solution}
